src/Noninterference/LoggedDisk/ATCD_TIE.v
@@ -1,0 +1,949 @@
+Require Import Eqdep Lia Framework FSParameters FileDiskLayer. (* LoggedDiskLayer TransactionCacheLayer TransactionalDiskLayer. *)
+Require Import FileDiskNoninterference FileDiskRefinement.
+Require Import ATC_ORS ATCDLayer ATC_Simulation HSS ATC_TransferProofs.
+Require Import ATCD_Simulation ATCD_AOE.
+Require Import Not_Init ATCD_ORS ATCD_TS.
+
+Import FileDiskLayer.
+Set Nested Proofs Allowed.
+
+
+Ltac destruct_and_split:=
+match goal with
+| [|- context [match ?x with | _ => _ end ] ] =>
+  destruct x
+end.
+
+
+Lemma TIE_auth_then_exec:
+    forall T (p1 p2: addr -> TD.(prog) (option T)) inum s1 s2 u ex,
+    (forall s1 s2,
+    refines_related ATC_Refinement (fun s1 s2  => exists s1a s2a, 
+    fst (snd s1) = Empty /\
+    fst (snd s2) = Empty /\
+    File.files_inner_rep s1a (fst (snd (snd s1))) /\ 
+    File.files_inner_rep s2a (fst (snd (snd s2))) /\ 
+    FD_related_states u ex s1a s2a) s1 s2 ->
+    transaction_input_equiv (lift_L2 AuthenticationOperation (p1 inum)) (lift_L2 AuthenticationOperation (p2 inum)) s1 s2) ->
+    
+    refines_related ATC_Refinement (AD_related_states u ex) s1 s2 ->
+    transaction_input_equiv (File.auth_then_exec inum p1) (File.auth_then_exec inum p2) s1 s2.
+    Proof.
+      unfold  refines_related, File.auth_then_exec in *; simpl; intuition eauto; cleanup.
+      {
+        Transparent Inode.get_owner.
+        unfold Inode.get_owner; simpl; intuition eauto.
+  
+        unfold Inode.InodeAllocator.read; simpl; intuition eauto.
+      destruct (Compare_dec.lt_dec inum
+      Inode.InodeAllocatorParams.num_of_blocks);
+      destruct (Compare_dec.lt_dec inum
+      Inode.InodeAllocatorParams.num_of_blocks); simpl; intuition eauto.
+      
+      {
+        unfold AD_related_states, refines_related in *; simpl in *; cleanup.
+        unfold refines, File.files_rep in *; simpl in *; cleanup.
+        unfold HC_refines in *; simpl in *; cleanup.
+        unfold TransactionToTransactionalDisk.Definitions.refines,
+        Transaction.transaction_rep in *; simpl in *; cleanup.
+        repeat split_ors; cleanup; try congruence.
+        repeat cleanup_pairs.
+        destruct s, s0; simpl in *; try lia; eauto.
+      }
+      {
+        unfold AD_related_states, refines_related in *; simpl in *; cleanup.
+        unfold refines, File.files_rep in *; simpl in *; cleanup.
+        unfold HC_refines in *; simpl in *; cleanup.
+        unfold TransactionToTransactionalDisk.Definitions.refines,
+        Transaction.transaction_rep in *; simpl in *; cleanup.
+        repeat split_ors; cleanup; try congruence.
+        repeat cleanup_pairs.
+        destruct s, s0; simpl in *; try lia; eauto.
+      }
+      unfold HC_refines in *; simpl in *; cleanup.
+      unfold TransactionToTransactionalDisk.Definitions.refines in *; simpl in *; cleanup.
+      repeat invert_lift2; cleanup.
+      eapply Transaction.read_finished in H8; eauto.
+      eapply Transaction.read_finished in H10; eauto.
+      cleanup. clear H10 H11.
+      destruct (nth_error (value_to_bits r1) inum);
+      destruct (nth_error (value_to_bits r2) inum);
+      simpl; intuition eauto.
+      destruct b, b0; simpl; intuition eauto.
+      {
+        unfold AD_related_states, refines_related in *; simpl in *; cleanup.
+        unfold refines, File.files_rep in *; simpl in *; cleanup.
+        unfold HC_refines in *; simpl in *; cleanup.
+        unfold TransactionToTransactionalDisk.Definitions.refines,
+        Transaction.transaction_rep in *; simpl in *; cleanup.
+        repeat split_ors; cleanup; try congruence.
+        repeat cleanup_pairs.
+        destruct s, s0; simpl in *; try lia; eauto.
+      }
+      {
+        unfold AD_related_states, refines_related in *; simpl in *; cleanup.
+        unfold refines, File.files_rep in *; simpl in *; cleanup.
+        unfold HC_refines in *; simpl in *; cleanup.
+        unfold TransactionToTransactionalDisk.Definitions.refines,
+        Transaction.transaction_rep in *; simpl in *; cleanup.
+        repeat split_ors; cleanup; try congruence.
+        repeat cleanup_pairs.
+        destruct s, s0; simpl in *; try lia; eauto.
+      }
+      destruct b; simpl; intuition eauto.
+      all: repeat destruct_and_split; simpl; eauto.
+      Opaque Inode.get_owner.
+    }
+    repeat destruct_and_split; simpl; eauto.
+    all: simpl; intuition eauto.
+    all: repeat destruct_and_split; simpl; intuition eauto.
+    all: repeat destruct_and_split; simpl; intuition eauto.
+    
+    eapply_fresh ATC_Simulation.ATC_oracle_refines_finished in H1; eauto; cleanup.
+    eapply_fresh ATC_Simulation.ATC_oracle_refines_finished in H2; eauto; cleanup.
+    
+    eapply_fresh ATC_Simulation.ATC_exec_lift_finished in H1; eauto;
+    try solve [apply TransactionToTransactionalDisk.Refinement.TC_to_TD_core_simulation_finished];
+    try solve [apply TransactionToTransactionalDisk.Refinement.TC_to_TD_core_simulation_crashed].
+    cleanup.
+    eapply_fresh ATC_Simulation.ATC_exec_lift_finished in H2; eauto;
+    try solve [apply TransactionToTransactionalDisk.Refinement.TC_to_TD_core_simulation_finished];
+    try solve [apply TransactionToTransactionalDisk.Refinement.TC_to_TD_core_simulation_crashed].
+    cleanup.
+
+    eapply_fresh ATC_ORS.ATC_oracle_refines_impl_eq in H8; eauto.
+    2: eapply have_same_structure_get_owner; eauto.
+    2: apply TD_oracle_refines_operation_eq.
+    cleanup.
+
+    repeat invert_lift2.
+    unfold AD_related_states, refines_related in *; simpl in *; cleanup.
+    unfold refines, File.files_rep, File.files_inner_rep in *; simpl in *; cleanup.
+    repeat cleanup_pairs.
+    eapply Inode.get_owner_finished in H14; eauto.
+    eapply Inode.get_owner_finished in H16; eauto.
+    cleanup; repeat split_ors; cleanup.
+    simpl in *.
+    repeat invert_exec; try congruence.
+
+    eapply H; eauto.
+    do 2 eexists; intuition eauto.
+    do 2 eexists; intuition eauto.
+    eexists; intuition eauto.
+    eexists; intuition eauto.
+    eapply File.DiskAllocator.block_allocator_rep_inbounds_eq; 
+    [| intros; FileInnerSpecs.solve_bounds ]; eauto.
+    eexists; intuition eauto.
+    eexists; intuition eauto.
+    eapply File.DiskAllocator.block_allocator_rep_inbounds_eq; 
+    [| intros; FileInnerSpecs.solve_bounds ]; eauto.
+
+    destruct p1; simpl; intuition eauto.
+    destruct o1; eauto.
+  Unshelve.
+  all: eauto.
+    Qed.
+
+    Lemma TIE_read_inner:
+    forall off inum u s0 s3,
+refines_related ATC_Refinement
+(fun s4 s5 : state AD =>
+ exists s1a s2a : disk File,
+ fst (snd s4) = Empty /\
+ fst (snd s5) = Empty /\
+   File.files_inner_rep s1a (fst (snd (snd s4))) /\
+   File.files_inner_rep s2a (fst (snd (snd s5))) /\
+   FD_related_states u None s1a s2a) s0 s3 ->
+transaction_input_equiv
+(@lift_L2 AuthenticationOperation _ TD _ (File.read_inner off inum))
+(@lift_L2 AuthenticationOperation _ TD _ (File.read_inner off inum)) s0 s3.
+Proof.
+      Transparent File.read_inner.  
+      unfold refines_related, File.read_inner; simpl; intuition eauto; cleanup.
+      {
+        Transparent Inode.get_block_number.
+        unfold Inode.get_block_number.
+        simpl; intuition eauto.
+        unfold Inode.InodeAllocator.read; simpl; intuition eauto.
+    destruct (Compare_dec.lt_dec inum
+    Inode.InodeAllocatorParams.num_of_blocks);
+    destruct (Compare_dec.lt_dec inum
+    Inode.InodeAllocatorParams.num_of_blocks); simpl; intuition eauto.
+    
+    {
+      unfold AD_related_states, refines_related in *; simpl in *; cleanup.
+      unfold refines, File.files_rep in *; simpl in *; cleanup.
+      unfold HC_refines in *; simpl in *; cleanup.
+      unfold TransactionToTransactionalDisk.Definitions.refines,
+      Transaction.transaction_rep in *; simpl in *; cleanup.
+      repeat split_ors; cleanup; try congruence.
+      repeat cleanup_pairs.
+      destruct s, s1; simpl in *; try lia; eauto.
+    }
+    {
+      unfold AD_related_states, refines_related in *; simpl in *; cleanup.
+      unfold refines, File.files_rep in *; simpl in *; cleanup.
+      unfold HC_refines in *; simpl in *; cleanup.
+      unfold TransactionToTransactionalDisk.Definitions.refines,
+      Transaction.transaction_rep in *; simpl in *; cleanup.
+      repeat split_ors; cleanup; try congruence.
+      repeat cleanup_pairs.
+      destruct s, s1; simpl in *; try lia; eauto.
+      }
+      unfold HC_refines in *; simpl in *; cleanup.
+      unfold TransactionToTransactionalDisk.Definitions.refines in *; simpl in *; cleanup.
+      repeat invert_lift2; cleanup.
+      eapply Transaction.read_finished in H11; eauto.
+      eapply Transaction.read_finished in H13; eauto.
+      cleanup. clear H13 H14.
+      destruct (nth_error (value_to_bits r1) inum);
+      destruct (nth_error (value_to_bits r2) inum);
+      simpl; intuition eauto.
+      destruct b, b0; simpl; intuition eauto.
+      {
+        unfold AD_related_states, refines_related in *; simpl in *; cleanup.
+        unfold refines, File.files_rep in *; simpl in *; cleanup.
+        unfold HC_refines in *; simpl in *; cleanup.
+        unfold TransactionToTransactionalDisk.Definitions.refines,
+        Transaction.transaction_rep in *; simpl in *; cleanup.
+        repeat split_ors; cleanup; try congruence.
+        repeat cleanup_pairs.
+        destruct s, s1; simpl in *; try lia; eauto.
+      }
+      {
+        unfold AD_related_states, refines_related in *; simpl in *; cleanup.
+        unfold refines, File.files_rep in *; simpl in *; cleanup.
+        unfold HC_refines in *; simpl in *; cleanup.
+        unfold TransactionToTransactionalDisk.Definitions.refines,
+        Transaction.transaction_rep in *; simpl in *; cleanup.
+        repeat split_ors; cleanup; try congruence.
+        repeat cleanup_pairs.
+        destruct s, s1; simpl in *; try lia; eauto.
+      }
+      destruct b; simpl; intuition eauto.
+      all: repeat destruct_and_split; simpl; eauto.
+      Opaque Inode.get_block_number.
+    }
+    repeat destruct_and_split; simpl; intuition eauto.
+    {
+      repeat cleanup_pairs.
+      eapply_fresh ATC_Simulation.ATC_oracle_refines_finished in H0; eauto; cleanup.
+      eapply_fresh ATC_Simulation.ATC_oracle_refines_finished in H1; eauto; cleanup.
+      
+      eapply_fresh ATC_Simulation.ATC_exec_lift_finished in H0; eauto;
+      try solve [apply TransactionToTransactionalDisk.Refinement.TC_to_TD_core_simulation_finished];
+      try solve [apply TransactionToTransactionalDisk.Refinement.TC_to_TD_core_simulation_crashed].
+      cleanup.
+      eapply_fresh ATC_Simulation.ATC_exec_lift_finished in H1; eauto;
+      try solve [apply TransactionToTransactionalDisk.Refinement.TC_to_TD_core_simulation_finished];
+      try solve [apply TransactionToTransactionalDisk.Refinement.TC_to_TD_core_simulation_crashed].
+      cleanup.
+  
+      eapply_fresh ATC_ORS.ATC_oracle_refines_impl_eq in H4; eauto.
+      2: eapply have_same_structure_get_block_number; eauto.
+      2: apply TD_oracle_refines_operation_eq.
+      cleanup.
+      repeat invert_lift2.
+      unfold AD_related_states, refines_related in *; simpl in *; cleanup.
+      unfold refines, File.files_rep, File.files_inner_rep in *; simpl in *; cleanup.
+      repeat cleanup_pairs.
+      eapply Inode.get_block_number_finished in H13; eauto.
+      eapply Inode.get_block_number_finished in H15; eauto.
+      cleanup; repeat split_ors; cleanup.
+      simpl in *; repeat cleanup_pairs.
+      {
+        clear H H2.
+        unfold File.DiskAllocator.read; simpl; intuition eauto.
+    destruct (Compare_dec.lt_dec
+    (seln (Inode.block_numbers x3) off 0)
+    File.DiskAllocatorParams.num_of_blocks);
+    destruct (Compare_dec.lt_dec
+    (seln (Inode.block_numbers x4) off 0)
+    File.DiskAllocatorParams.num_of_blocks); simpl; intuition eauto.
+    
+    {
+      unfold AD_related_states, refines_related in *; simpl in *; cleanup.
+      unfold refines, File.files_rep in *; simpl in *; cleanup.
+      unfold HC_refines in *; simpl in *; cleanup.
+      unfold TransactionToTransactionalDisk.Definitions.refines,
+      Transaction.transaction_rep in *; simpl in *; cleanup.
+      repeat split_ors; cleanup; try congruence.
+      repeat cleanup_pairs.
+      destruct s, s2; simpl in *; try lia; eauto.
+    }
+    {
+      unfold AD_related_states, refines_related in *; simpl in *; cleanup.
+      unfold refines, File.files_rep in *; simpl in *; cleanup.
+      unfold HC_refines in *; simpl in *; cleanup.
+      unfold TransactionToTransactionalDisk.Definitions.refines,
+      Transaction.transaction_rep in *; simpl in *; cleanup.
+      repeat split_ors; cleanup; try congruence.
+      repeat cleanup_pairs.
+      destruct s, s2; simpl in *; try lia; eauto.
+    }
+      unfold HC_refines in *; simpl in *; cleanup.
+      unfold TransactionToTransactionalDisk.Definitions.refines in *; simpl in *; cleanup.
+      repeat invert_lift2; cleanup.
+      eapply Transaction.read_finished in H11; eauto.
+      eapply Transaction.read_finished in H24; eauto.
+      cleanup. clear H24 H25.
+      destruct (nth_error (value_to_bits r1) (seln (Inode.block_numbers x3) off 0));
+      destruct (nth_error (value_to_bits r2) (seln (Inode.block_numbers x4) off 0));
+      simpl; intuition eauto.
+      destruct b, b0; simpl; intuition eauto.
+      {
+        eapply data_block_inbounds.
+        4: eauto.
+        all: eauto.
+        eapply File.DiskAllocator.block_allocator_rep_inbounds_eq; 
+        [| intros; FileInnerSpecs.solve_bounds ]; eauto.
+      }
+      {
+        eapply data_block_inbounds.
+        4: eauto.
+        all: eauto.
+        eapply File.DiskAllocator.block_allocator_rep_inbounds_eq; 
+        [| intros; FileInnerSpecs.solve_bounds ]; eauto.
+      }
+      {
+        unfold AD_related_states, refines_related in *; simpl in *; cleanup.
+        unfold refines, File.files_rep in *; simpl in *; cleanup.
+        unfold HC_refines in *; simpl in *; cleanup.
+        unfold TransactionToTransactionalDisk.Definitions.refines,
+        Transaction.transaction_rep in *; simpl in *; cleanup.
+        repeat split_ors; cleanup; try congruence.
+        repeat cleanup_pairs.
+        destruct s, s2; simpl in *; try lia; eauto.
+      }
+      {
+        unfold AD_related_states, refines_related in *; simpl in *; cleanup.
+        unfold refines, File.files_rep in *; simpl in *; cleanup.
+        unfold HC_refines in *; simpl in *; cleanup.
+        unfold TransactionToTransactionalDisk.Definitions.refines,
+        Transaction.transaction_rep in *; simpl in *; cleanup.
+        repeat split_ors; cleanup; try congruence.
+        repeat cleanup_pairs.
+        destruct s, s2; simpl in *; try lia; eauto.
+      }
+      destruct b; simpl; intuition eauto.
+    }
+  }
+  repeat destruct_and_split; simpl; eauto.
+  Unshelve.
+  all: eauto.
+Qed.
+
+
+Lemma TIE_write_inner:
+    forall off inum u s0 s3 v,
+refines_related ATC_Refinement
+(fun s4 s5 : state AD =>
+ exists s1a s2a : disk File,
+ fst (snd s4) = Empty /\
+ fst (snd s5) = Empty /\
+   File.files_inner_rep s1a (fst (snd (snd s4))) /\
+   File.files_inner_rep s2a (fst (snd (snd s5))) /\
+   FD_related_states u None s1a s2a) s0 s3 ->
+transaction_input_equiv
+(@lift_L2 AuthenticationOperation _ TD _ (File.write_inner off v inum))
+(@lift_L2 AuthenticationOperation _ TD _ (File.write_inner off v inum)) s0 s3.
+Proof.
+      Transparent File.write_inner.  
+      unfold refines_related, File.write_inner; simpl; intuition eauto; cleanup.
+      {
+        Transparent Inode.get_block_number.
+        unfold Inode.get_block_number.
+        simpl; intuition eauto.
+        unfold Inode.InodeAllocator.read; simpl; intuition eauto.
+    destruct (Compare_dec.lt_dec inum
+    Inode.InodeAllocatorParams.num_of_blocks);
+    destruct (Compare_dec.lt_dec inum
+    Inode.InodeAllocatorParams.num_of_blocks); simpl; intuition eauto.
+    
+    {
+      unfold AD_related_states, refines_related in *; simpl in *; cleanup.
+      unfold refines, File.files_rep in *; simpl in *; cleanup.
+      unfold HC_refines in *; simpl in *; cleanup.
+      unfold TransactionToTransactionalDisk.Definitions.refines,
+      Transaction.transaction_rep in *; simpl in *; cleanup.
+      repeat split_ors; cleanup; try congruence.
+      repeat cleanup_pairs.
+      destruct s, s1; simpl in *; try lia; eauto.
+    }
+    {
+      unfold AD_related_states, refines_related in *; simpl in *; cleanup.
+      unfold refines, File.files_rep in *; simpl in *; cleanup.
+      unfold HC_refines in *; simpl in *; cleanup.
+      unfold TransactionToTransactionalDisk.Definitions.refines,
+      Transaction.transaction_rep in *; simpl in *; cleanup.
+      repeat split_ors; cleanup; try congruence.
+      repeat cleanup_pairs.
+      destruct s, s1; simpl in *; try lia; eauto.
+    }
+    unfold HC_refines in *; simpl in *; cleanup.
+    unfold TransactionToTransactionalDisk.Definitions.refines in *; simpl in *; cleanup.
+    repeat invert_lift2; cleanup.
+    eapply Transaction.read_finished in H11; eauto.
+    eapply Transaction.read_finished in H13; eauto.
+    cleanup. clear H13 H14.
+    destruct (nth_error (value_to_bits r1) inum);
+    destruct (nth_error (value_to_bits r2) inum);
+    simpl; intuition eauto.
+    destruct b, b0; simpl; intuition eauto.
+    {
+      unfold AD_related_states, refines_related in *; simpl in *; cleanup.
+      unfold refines, File.files_rep in *; simpl in *; cleanup.
+      unfold HC_refines in *; simpl in *; cleanup.
+      unfold TransactionToTransactionalDisk.Definitions.refines,
+      Transaction.transaction_rep in *; simpl in *; cleanup.
+      repeat split_ors; cleanup; try congruence.
+      repeat cleanup_pairs.
+      destruct s, s1; simpl in *; try lia; eauto.
+    }
+    {
+      unfold AD_related_states, refines_related in *; simpl in *; cleanup.
+      unfold refines, File.files_rep in *; simpl in *; cleanup.
+      unfold HC_refines in *; simpl in *; cleanup.
+      unfold TransactionToTransactionalDisk.Definitions.refines,
+      Transaction.transaction_rep in *; simpl in *; cleanup.
+      repeat split_ors; cleanup; try congruence.
+      repeat cleanup_pairs.
+      destruct s, s1; simpl in *; try lia; eauto.
+    }
+    destruct b; simpl; intuition eauto.
+    all: repeat destruct_and_split; simpl; eauto.
+    Opaque Inode.get_block_number.
+  }
+    repeat destruct_and_split; simpl; intuition eauto.
+    {
+      repeat cleanup_pairs.
+      eapply_fresh ATC_Simulation.ATC_oracle_refines_finished in H0; eauto; cleanup.
+      eapply_fresh ATC_Simulation.ATC_oracle_refines_finished in H1; eauto; cleanup.
+      
+      eapply_fresh ATC_Simulation.ATC_exec_lift_finished in H0; eauto;
+      try solve [apply TransactionToTransactionalDisk.Refinement.TC_to_TD_core_simulation_finished];
+      try solve [apply TransactionToTransactionalDisk.Refinement.TC_to_TD_core_simulation_crashed].
+      cleanup.
+      eapply_fresh ATC_Simulation.ATC_exec_lift_finished in H1; eauto;
+      try solve [apply TransactionToTransactionalDisk.Refinement.TC_to_TD_core_simulation_finished];
+      try solve [apply TransactionToTransactionalDisk.Refinement.TC_to_TD_core_simulation_crashed].
+      cleanup.
+  
+      eapply_fresh ATC_ORS.ATC_oracle_refines_impl_eq in H4; eauto.
+      2: eapply have_same_structure_get_block_number; eauto.
+      2: apply TD_oracle_refines_operation_eq.
+      cleanup.
+      repeat invert_lift2.
+      unfold AD_related_states, refines_related in *; simpl in *; cleanup.
+      unfold refines, File.files_rep, File.files_inner_rep in *; simpl in *; cleanup.
+      repeat cleanup_pairs.
+      eapply Inode.get_block_number_finished in H13; eauto.
+      eapply Inode.get_block_number_finished in H15; eauto.
+      cleanup; repeat split_ors; cleanup.
+      simpl in *; repeat cleanup_pairs.
+      {
+        clear H H2.
+        unfold File.DiskAllocator.write; simpl; intuition eauto.
+    destruct (Compare_dec.lt_dec
+    (seln (Inode.block_numbers x3) off 0)
+    File.DiskAllocatorParams.num_of_blocks);
+    destruct (Compare_dec.lt_dec
+    (seln (Inode.block_numbers x4) off 0)
+    File.DiskAllocatorParams.num_of_blocks); simpl; intuition eauto.
+    
+    {
+      unfold AD_related_states, refines_related in *; simpl in *; cleanup.
+      unfold refines, File.files_rep in *; simpl in *; cleanup.
+      unfold HC_refines in *; simpl in *; cleanup.
+      unfold TransactionToTransactionalDisk.Definitions.refines,
+      Transaction.transaction_rep in *; simpl in *; cleanup.
+      repeat split_ors; cleanup; try congruence.
+      repeat cleanup_pairs.
+      destruct s, s2; simpl in *; try lia; eauto.
+    }
+    {
+      unfold AD_related_states, refines_related in *; simpl in *; cleanup.
+      unfold refines, File.files_rep in *; simpl in *; cleanup.
+      unfold HC_refines in *; simpl in *; cleanup.
+      unfold TransactionToTransactionalDisk.Definitions.refines,
+      Transaction.transaction_rep in *; simpl in *; cleanup.
+      repeat split_ors; cleanup; try congruence.
+      repeat cleanup_pairs.
+      destruct s, s2; simpl in *; try lia; eauto.
+    }
+      unfold HC_refines in *; simpl in *; cleanup.
+      unfold TransactionToTransactionalDisk.Definitions.refines in *; simpl in *; cleanup.
+      repeat invert_lift2; cleanup.
+      eapply Transaction.read_finished in H11; eauto.
+      eapply Transaction.read_finished in H24; eauto.
+      cleanup. clear H24 H25.
+      destruct (nth_error (value_to_bits r1) (seln (Inode.block_numbers x3) off 0));
+      destruct (nth_error (value_to_bits r2) (seln (Inode.block_numbers x4) off 0));
+      simpl; intuition eauto.
+      destruct b, b0; simpl; intuition eauto.
+      {
+        eapply data_block_inbounds.
+        4: eauto.
+        all: eauto.
+        eapply File.DiskAllocator.block_allocator_rep_inbounds_eq; 
+        [| intros; FileInnerSpecs.solve_bounds ]; eauto.
+      }
+      {
+        eapply data_block_inbounds.
+        4: eauto.
+        all: eauto.
+        eapply File.DiskAllocator.block_allocator_rep_inbounds_eq; 
+        [| intros; FileInnerSpecs.solve_bounds ]; eauto.
+      }
+      {
+        unfold AD_related_states, refines_related in *; simpl in *; cleanup.
+        unfold refines, File.files_rep in *; simpl in *; cleanup.
+        unfold HC_refines in *; simpl in *; cleanup.
+        unfold TransactionToTransactionalDisk.Definitions.refines,
+        Transaction.transaction_rep in *; simpl in *; cleanup.
+        repeat split_ors; cleanup; try congruence.
+        repeat cleanup_pairs.
+        destruct s, s2; simpl in *; try lia; eauto.
+        erewrite addr_list_to_blocks_length_eq; eauto.
+      }
+      {
+        unfold AD_related_states, refines_related in *; simpl in *; cleanup.
+        unfold refines, File.files_rep in *; simpl in *; cleanup.
+        unfold HC_refines in *; simpl in *; cleanup.
+        unfold TransactionToTransactionalDisk.Definitions.refines,
+        Transaction.transaction_rep in *; simpl in *; cleanup.
+        repeat split_ors; cleanup; try congruence.
+        repeat cleanup_pairs.
+        destruct s, s2; simpl in *; try lia; eauto.
+        erewrite addr_list_to_blocks_length_eq; eauto.
+      }
+      destruct b; simpl; intuition eauto.
+    }
+  }
+  unfold File.DiskAllocator.write;
+  repeat destruct_and_split; simpl; eauto.
+  Unshelve.
+  all: eauto.
+Qed.
+
+
+Lemma TIE_create:
+    forall u' s1 s2 v,
+refines_related ATC_Refinement
+  (AD_related_states u' None) s1 s2 ->
+transaction_input_equiv
+(File.create v) (File.create v) s1 s2.
+Proof.
+Transparent File.create.  
+unfold refines_related, File.create; simpl; intuition eauto; cleanup.
+{
+  Transparent Inode.alloc.
+  unfold Inode.alloc.
+  simpl; intuition eauto.
+  {
+    unfold AD_related_states, refines_related in *; simpl in *; cleanup.
+    unfold refines, File.files_rep in *; simpl in *; cleanup.
+    unfold HC_refines in *; simpl in *; cleanup.
+    unfold TransactionToTransactionalDisk.Definitions.refines,
+    Transaction.transaction_rep in *; simpl in *; cleanup.
+    repeat split_ors; cleanup; try congruence.
+    repeat cleanup_pairs.
+    destruct s, s0; simpl in *; try lia; eauto.
+  }
+  {
+    unfold AD_related_states, refines_related in *; simpl in *; cleanup.
+    unfold refines, File.files_rep in *; simpl in *; cleanup.
+    unfold HC_refines in *; simpl in *; cleanup.
+    unfold TransactionToTransactionalDisk.Definitions.refines,
+    Transaction.transaction_rep in *; simpl in *; cleanup.
+    repeat split_ors; cleanup; try congruence.
+    repeat cleanup_pairs.
+    destruct s, s0; simpl in *; try lia; eauto.
+  }
+  unfold HC_refines in *; simpl in *; cleanup.
+  unfold TransactionToTransactionalDisk.Definitions.refines in *; simpl in *; cleanup.
+  repeat invert_lift2; cleanup.
+  eapply Transaction.read_finished in H7; eauto.
+  eapply Transaction.read_finished in H9; eauto.
+  cleanup.
+
+  destruct_fresh (Compare_dec.lt_dec
+  (get_first_zero_index
+      (firstn
+        Inode.InodeAllocatorParams.num_of_blocks
+        (value_to_bits r1)))
+  Inode.InodeAllocatorParams.num_of_blocks);
+  destruct_fresh (Compare_dec.lt_dec
+  (get_first_zero_index
+      (firstn
+        Inode.InodeAllocatorParams.num_of_blocks
+        (value_to_bits r2)))
+  Inode.InodeAllocatorParams.num_of_blocks);
+  simpl; eauto. 
+  FileSpecs.hide H9.
+  FileSpecs.hide H10.
+  intuition eauto; try lia.
+  cleanup.
+  {
+    pose proof Inode.InodeAllocatorParams.blocks_fit_in_disk.
+    unfold Inode.InodeAllocatorParams.bitmap_addr,
+    Inode.InodeAllocatorParams.num_of_blocks in *; lia.
+  }
+  {
+    pose proof Inode.InodeAllocatorParams.blocks_fit_in_disk.
+    unfold Inode.InodeAllocatorParams.bitmap_addr,
+    Inode.InodeAllocatorParams.num_of_blocks in *; lia.
+  }
+  {
+    unfold AD_related_states, refines_related in *; simpl in *; cleanup.
+    unfold refines, File.files_rep in *; simpl in *; cleanup.
+    unfold HC_refines in *; simpl in *; cleanup.
+    unfold TransactionToTransactionalDisk.Definitions.refines,
+    Transaction.transaction_rep in *; simpl in *; cleanup.
+    repeat split_ors; cleanup; try congruence.
+    repeat cleanup_pairs.
+    destruct s, s0; simpl in *; try lia; eauto.
+    erewrite addr_list_to_blocks_length_eq; eauto.
+  }
+  {
+    unfold AD_related_states, refines_related in *; simpl in *; cleanup.
+    unfold refines, File.files_rep in *; simpl in *; cleanup.
+    unfold HC_refines in *; simpl in *; cleanup.
+    unfold TransactionToTransactionalDisk.Definitions.refines,
+    Transaction.transaction_rep in *; simpl in *; cleanup.
+    repeat split_ors; cleanup; try congruence.
+    repeat cleanup_pairs.
+    destruct s, s0; simpl in *; try lia; eauto.
+    erewrite addr_list_to_blocks_length_eq; eauto.
+  }
+
+  repeat cleanup_pairs.
+  unfold HC_refines in *; simpl in *; cleanup.
+  unfold TransactionToTransactionalDisk.Definitions.refines in *; simpl in *; cleanup.
+  repeat invert_lift2; cleanup.
+  eapply Transaction.write_finished in H2; eauto.
+  eapply Transaction.write_finished in H8; eauto.
+  cleanup.
+  FileSpecs.hide H2.
+  FileSpecs.hide H8.
+
+  unfold AD_related_states, refines_related in *; simpl in *; cleanup.
+  unfold refines, File.files_rep in *; simpl in *; cleanup.
+  unfold HC_refines in *; simpl in *; cleanup.
+  unfold TransactionToTransactionalDisk.Definitions.refines,
+  Transaction.transaction_rep in H4, H5; simpl in *; cleanup.
+  repeat split_ors; cleanup; try congruence.
+  repeat cleanup_pairs.
+  destruct s, s1; simpl in *; try lia; eauto.
+
+  FileSpecs.reveal H2.
+  FileSpecs.reveal H8.
+  repeat split_ors; cleanup; try lia; simpl in *; eauto.
+
+  intuition eauto; try solve [
+  erewrite addr_list_to_blocks_length_eq; eauto].
+  repeat destruct_and_split; simpl; intuition eauto.
+}
+repeat destruct_and_split; simpl; intuition eauto.
+Qed.
+
+Lemma TIE_extend_inner:
+    forall inum u s0 s3 v,
+refines_related ATC_Refinement
+(fun s4 s5 : state AD =>
+ exists s1a s2a : disk File,
+ fst (snd s4) = Empty /\
+ fst (snd s5) = Empty /\
+   File.files_inner_rep s1a (fst (snd (snd s4))) /\
+   File.files_inner_rep s2a (fst (snd (snd s5))) /\
+   FD_related_states u None s1a s2a) s0 s3 ->
+transaction_input_equiv
+(@lift_L2 AuthenticationOperation _ TD _ (File.extend_inner v inum))
+(@lift_L2 AuthenticationOperation _ TD _ (File.extend_inner v inum)) s0 s3.
+Proof.
+  Transparent File.extend_inner.  
+  Opaque File.DiskAllocator.alloc.
+  unfold refines_related, File.extend_inner; simpl; intuition eauto; cleanup.
+{
+  Transparent File.DiskAllocator.alloc.
+  simpl; intuition eauto.
+  {
+    unfold AD_related_states, refines_related in *; simpl in *; cleanup.
+    unfold refines, File.files_rep in *; simpl in *; cleanup.
+    unfold HC_refines in *; simpl in *; cleanup.
+    unfold TransactionToTransactionalDisk.Definitions.refines,
+    Transaction.transaction_rep in *; simpl in *; cleanup.
+    repeat split_ors; cleanup; try congruence.
+    repeat cleanup_pairs.
+    destruct s, s1; simpl in *; try lia; eauto.
+  }
+  {
+    unfold AD_related_states, refines_related in *; simpl in *; cleanup.
+    unfold refines, File.files_rep in *; simpl in *; cleanup.
+    unfold HC_refines in *; simpl in *; cleanup.
+    unfold TransactionToTransactionalDisk.Definitions.refines,
+    Transaction.transaction_rep in *; simpl in *; cleanup.
+    repeat split_ors; cleanup; try congruence.
+    repeat cleanup_pairs.
+    destruct s, s1; simpl in *; try lia; eauto.
+  }
+
+  unfold HC_refines in *; simpl in *; cleanup.
+  unfold TransactionToTransactionalDisk.Definitions.refines in *; simpl in *; cleanup.
+  repeat invert_lift2; cleanup.
+  eapply Transaction.read_finished in H11; eauto.
+  eapply Transaction.read_finished in H13; eauto.
+  cleanup. clear H13 H14.
+  destruct (Compare_dec.lt_dec
+  (get_first_zero_index
+    (firstn
+        File.DiskAllocatorParams.num_of_blocks
+        (value_to_bits r1)))
+  File.DiskAllocatorParams.num_of_blocks);
+  destruct (Compare_dec.lt_dec
+  (get_first_zero_index
+    (firstn
+        File.DiskAllocatorParams.num_of_blocks
+        (value_to_bits r2)))
+  File.DiskAllocatorParams.num_of_blocks);
+  simpl; intuition eauto.
+  {
+    pose proof File.DiskAllocatorParams.blocks_fit_in_disk.
+    unfold File.DiskAllocatorParams.bitmap_addr,
+    File.DiskAllocatorParams.num_of_blocks in *.
+    lia.
+  }
+  {
+    pose proof File.DiskAllocatorParams.blocks_fit_in_disk.
+    unfold File.DiskAllocatorParams.bitmap_addr,
+    File.DiskAllocatorParams.num_of_blocks in *.
+    lia.
+  }
+  {
+    unfold AD_related_states, refines_related in *; simpl in *; cleanup.
+    unfold refines, File.files_rep in *; simpl in *; cleanup.
+    unfold HC_refines in *; simpl in *; cleanup.
+    unfold TransactionToTransactionalDisk.Definitions.refines,
+    Transaction.transaction_rep in *; simpl in *; cleanup.
+    repeat split_ors; cleanup; try congruence.
+    repeat cleanup_pairs.
+    destruct s, s1; simpl in *; try lia; eauto.
+    erewrite addr_list_to_blocks_length_eq; eauto.
+  }
+  {
+    unfold AD_related_states, refines_related in *; simpl in *; cleanup.
+    unfold refines, File.files_rep in *; simpl in *; cleanup.
+    unfold HC_refines in *; simpl in *; cleanup.
+    unfold TransactionToTransactionalDisk.Definitions.refines,
+    Transaction.transaction_rep in *; simpl in *; cleanup.
+    repeat split_ors; cleanup; try congruence.
+    repeat cleanup_pairs.
+    destruct s, s1; simpl in *; try lia; eauto.
+    erewrite addr_list_to_blocks_length_eq; eauto.
+  }
+  repeat cleanup_pairs; simpl in *.
+
+  unfold HC_refines in *; simpl in *; cleanup.
+  unfold TransactionToTransactionalDisk.Definitions.refines in *; simpl in *; cleanup.
+  repeat invert_lift2; cleanup.
+  eapply Transaction.write_finished in H1; eauto.
+  eapply Transaction.write_finished in H10; eauto.
+  unfold AD_related_states, refines_related in *; simpl in *; cleanup.
+  unfold refines, File.files_rep in *; simpl in *; cleanup.
+  unfold HC_refines in *; simpl in *; cleanup.
+  unfold TransactionToTransactionalDisk.Definitions.refines,
+  Transaction.transaction_rep in *; simpl in *; cleanup.
+  FileSpecs.hide H1.
+  FileSpecs.hide H10.
+  repeat split_ors; cleanup; try congruence.
+  repeat cleanup_pairs.
+  destruct s, s4; simpl in *; try lia; eauto.
+  FileSpecs.reveal H1.
+  FileSpecs.reveal H10.
+  cleanup.
+  {
+    repeat (repeat split_ors; cleanup; try congruence); simpl in *; eauto.
+    simpl; intuition eauto; 
+    try solve [erewrite addr_list_to_blocks_length_eq; eauto].
+    repeat destruct_and_split; simpl; intuition eauto.
+  }
+}
+repeat destruct_and_split; simpl; intuition eauto.
+{
+   (***********)
+   unfold HC_refines in *; simpl in *; cleanup.
+    unfold TransactionToTransactionalDisk.Definitions.refines in *; simpl in *; cleanup.
+    unfold File.DiskAllocator.alloc in *; simpl in *.
+    repeat invert_exec_no_match;
+    eapply Transaction.read_finished in H12; eauto;
+    eapply Transaction.read_finished in H15; eauto;
+    cleanup; try lia; repeat cleanup_pairs;
+    repeat (simpl in *; repeat invert_exec_no_match; cleanup).
+    {
+      simpl in *.
+      clear H16 H17.
+      eapply Transaction.write_finished in H2; eauto;
+      eapply Transaction.write_finished in H10; eauto;
+      cleanup; try lia; repeat cleanup_pairs;
+      repeat split_ors; cleanup; try congruence.
+      eapply Transaction.write_finished in H3; eauto;
+      eapply Transaction.write_finished in H12; eauto;
+      cleanup; try lia; repeat cleanup_pairs;
+      repeat split_ors; cleanup; try congruence.
+      
+      unfold TransactionToTransactionalDisk.Definitions.refines,
+      Transaction.transaction_rep in H8, H9; simpl in *; cleanup.
+      repeat split_ors; cleanup; try congruence.
+      repeat cleanup_pairs.
+      destruct s, s2; simpl in *; try lia; eauto.
+      {
+        Transparent Inode.extend.
+        Opaque Inode.get_inode.
+        unfold Inode.extend; simpl; intuition.
+        {
+          Transparent Inode.get_inode.
+          simpl; intuition.
+          unfold Inode.InodeAllocator.read; simpl; intuition eauto.
+          destruct (Compare_dec.lt_dec inum
+          Inode.InodeAllocatorParams.num_of_blocks);
+          destruct (Compare_dec.lt_dec inum
+          Inode.InodeAllocatorParams.num_of_blocks); 
+          simpl; intuition eauto.
+          cleanup; eauto; try congruence.
+          destruct (addr_eq_dec Inode.InodeAllocatorParams.bitmap_addr
+          (File.DiskAllocatorParams.bitmap_addr +
+          S
+            (get_first_zero_index
+                (firstn File.DiskAllocatorParams.num_of_blocks
+                  (value_to_bits x6))))); eauto.
+          shelve.
+          cleanup; eauto; try congruence.
+          destruct (addr_eq_dec Inode.InodeAllocatorParams.bitmap_addr
+          (File.DiskAllocatorParams.bitmap_addr +
+          S
+            (get_first_zero_index
+                (firstn File.DiskAllocatorParams.num_of_blocks
+                  (value_to_bits x11))))); eauto.
+          shelve.
+        
+          {
+            unfold HC_refines in *; simpl in *; cleanup.
+            unfold TransactionToTransactionalDisk.Definitions.refines in *; simpl in *; cleanup.
+            repeat invert_lift2; cleanup.
+            eapply Transaction.read_finished in H16; eauto.
+            eapply Transaction.read_finished in H19; eauto.
+            cleanup. clear H19 H20.
+            destruct (nth_error (value_to_bits r1) inum);
+            destruct (nth_error (value_to_bits r2) inum);
+            simpl; intuition eauto.
+            destruct b, b0; simpl; intuition eauto.
+            {
+              unfold AD_related_states, refines_related in *; simpl in *; cleanup.
+              unfold refines, File.files_rep in *; simpl in *; cleanup.
+              destruct (addr_eq_dec
+              (Inode.InodeAllocatorParams.bitmap_addr + S inum)
+              (File.DiskAllocatorParams.bitmap_addr +
+              S
+                (get_first_zero_index
+                    (firstn
+                      File.DiskAllocatorParams.num_of_blocks
+                      (value_to_bits x6))))); eauto.
+              shelve.
+            }
+            {
+              unfold AD_related_states, refines_related in *; simpl in *; cleanup.
+              unfold refines, File.files_rep in *; simpl in *; cleanup.
+              destruct (addr_eq_dec
+              (Inode.InodeAllocatorParams.bitmap_addr + S inum)
+              (File.DiskAllocatorParams.bitmap_addr +
+              S
+                (get_first_zero_index
+                    (firstn
+                      File.DiskAllocatorParams.num_of_blocks
+                      (value_to_bits x11))))); eauto.
+              shelve.
+            }
+            destruct b; simpl; intuition eauto.
+            
+          }
+          repeat destruct_and_split; simpl; eauto.
+        }
+        {
+          repeat destruct_and_split; simpl; eauto.
+          unfold Inode.get_inode in *; simpl in *;
+          repeat (repeat invert_exec; simpl in *; cleanup).
+          unfold Inode.InodeAllocator.read in *; simpl in *;
+          repeat (repeat invert_exec; simpl in *; cleanup).
+          eapply Transaction.read_finished in H21; eauto.
+          eapply Transaction.read_finished in H18; eauto.
+          cleanup. clear H18 H22.
+          eapply Transaction.read_finished in H8; eauto.
+          eapply Transaction.read_finished in H19; eauto.
+          cleanup. clear H19 H22.
+          repeat cleanup_pairs.
+          unfold Inode.set_inode; simpl; intuition eauto.
+          unfold Inode.InodeAllocator.write; simpl; intuition eauto.
+          destruct (Compare_dec.lt_dec inum
+          Inode.InodeAllocatorParams.num_of_blocks); try lia.
+          simpl; intuition eauto.
+          {
+            cleanup; eauto; try congruence.
+          destruct (addr_eq_dec Inode.InodeAllocatorParams.bitmap_addr
+          (File.DiskAllocatorParams.bitmap_addr +
+          S
+            (get_first_zero_index
+                (firstn File.DiskAllocatorParams.num_of_blocks
+                  (value_to_bits x6))))); eauto.
+          shelve.
+          }
+          {
+          cleanup; eauto; try congruence.
+          destruct (addr_eq_dec Inode.InodeAllocatorParams.bitmap_addr
+          (File.DiskAllocatorParams.bitmap_addr +
+          S
+            (get_first_zero_index
+                (firstn File.DiskAllocatorParams.num_of_blocks
+                  (value_to_bits x11))))); eauto.
+          shelve.
+          }
+          unfold HC_refines in *; simpl in *; cleanup.
+            unfold TransactionToTransactionalDisk.Definitions.refines in *; simpl in *; cleanup.
+            repeat invert_lift2; cleanup.
+            eapply Transaction.read_finished in H16; eauto.
+            eapply Transaction.read_finished in H19; eauto.
+            cleanup. clear H19 H21.
+            destruct (nth_error (value_to_bits r1) inum);
+            destruct (nth_error (value_to_bits r2) inum);
+            simpl; intuition eauto.
+            destruct b, b0; simpl; intuition eauto.
+            {
+              unfold AD_related_states, refines_related in *; simpl in *; cleanup.
+              unfold refines, File.files_rep in *; simpl in *; cleanup.
+              erewrite addr_list_to_blocks_length_eq; eauto.
+            }
+            {
+              unfold AD_related_states, refines_related in *; simpl in *; cleanup.
+              unfold refines, File.files_rep in *; simpl in *; cleanup.
+              erewrite addr_list_to_blocks_length_eq; eauto.
+            }
+            destruct b; simpl; intuition eauto.
+            {
+              unfold Inode.set_inode; simpl; intuition eauto.
+              unfold Inode.InodeAllocator.write; simpl; intuition eauto.
+              destruct (Compare_dec.lt_dec inum
+              Inode.InodeAllocatorParams.num_of_blocks); simpl; intuition eauto.
+            }
+          }
+        }
+      }
+    }
+    {
+      unfold Inode.extend; simpl; intuition eauto.
+    }
+    Unshelve.
+    all:
+      unfold Inode.InodeAllocatorParams.bitmap_addr,
+      File.DiskAllocatorParams.bitmap_addr,
+      Inode.InodeAllocatorParams.num_of_blocks in *;
+      pose proof inodes_before_data; try lia.
+Qed.
